Setting up the context of spatial graph in logic level.

data_structure/spatial_graph.v
@@ -1,1 +1,40 @@
+Require Import VST.msl.seplog.
+Require Import RamifyCoq.msl_ext.abs_addr.
+Require Import RamifyCoq.msl_ext.seplog.
+
+Class SPATIAL_GRAPH_SET_UP: Type := {
+  Data: Type;
+  addr: Type;
+  addr_eq_dec: forall x y: addr, {x = y} + {x <> y};
+  addr_eqb: addr -> addr -> bool := fun x y => if addr_eq_dec x y then true else false
+}.
+
+Instance AV_SGraph `{SPATIAL_GRAPH_SET_UP} : AbsAddr.
+  apply (mkAbsAddr addr (Data * addr * addr) (fun x y => addr_eqb x y)); simpl; intros.
+  + unfold addr_eqb.
+    destruct (addr_eq_dec p1 p2), (addr_eq_dec p2 p1); try congruence.
+  + unfold addr_eqb in H0.
+    destruct (addr_eq_dec p1 p1); congruence.
+Defined.
+
+Section SPATIAL_GRAPH.
+
+Variable A: Type.
+Variable ND: NatDed A.
+Variable SL : SepLog A.
+Variable ClSL: ClassicalSep A.
+Variable PSL : PreciseSepLog A.
+Variable CoSL: CorableSepLog A.
+Variable OSL: OverlapSepLog A.
+Variable DSL : DisjointedSepLog A.
+
+Variable spatial_graph_set_up: SPATIAL_GRAPH_SET_UP.
+Variable trinode : addr -> (Data * addr * addr) -> A.
+Variable MSL: MapstoSepLog AV_SGraph trinode.
+Variable sMSL: StaticMapstoSepLog AV_SGraph trinode.
+Variable nMSL: NormalMapstoSepLog AV_SGraph trinode.
+
+(* Now start proof here. *)
+
+End SPATIAL_GRAPH.
 
